
But here's an example from a "true" result where the model guess into becoming right:

#+begin_example
#### 2.1 Simplify `((( )))`

`((( )))` is three nested pairs: `(((( ))))` is actually:

- Innermost: `()`  
- Next: `(())` \u2192 by I2 \u2192 void  
- So `((()))` becomes `(void)` \u2192 `()`  
- Then `(((())))` is one more layer: `(())` again \u2192 void

So:
- `((( )))` \u2192 `(((())))` \u2192 void
#+end_example

See the error? The model suddenly hallucinated "three nested pairs ((( )))" -> "((((  ))))" -> "void". 


Additionally a common failure mode I see in "false" results:
#+begin_example
### Step 1: Simplify each inner `(())` using I2 (Order)

Axiom I2: `(()) = void`

So each `(())` becomes `void`:

3. `( (()) (()) ) \u2192 ( void void )`

But `void` is just \"nothing,\" so `( void void )` is the same as having two adjacent marks inside the outer pair:

4. `( void void ) = ( () () )`
#+end_example

Catch that? It mistook the idea that =void void= is the same as having two adjacent marks: =() ()=.

Another common failure mode I see is also comes from transcribing =void= -> =(void)=. Sometimes this leads to mistakes like believing that =void void= -> =(void) (void)=.

#+begin_example
"Start with the expression:

1. Expression:  
   `()(())`

2. Focus on the right part `(())`.  
   By Axiom I2 (Order):  
   `(()) = void`

3. Substitute back into the expression:  
   `()(()) = ()(void)`

4. In Laws of Form, concatenation with void contributes nothing, so:  
   `()(void) = ()`

So the expression simplifies to a single mark.

FINAL: ()""
#+end_example

In this case, the derivation was largely correct, although notationally =(void)= is highly sus.

In these examples, even if the final answer was correct, the /reasoning is incorrect/. Do I try to catch incorrect intermediate results? How do I classify this? I was thinking that this should be considered a "false positive".
